lib/examples/vertex_simple.ml
@@ -1,10 +1,10 @@
 let main ~num_worker a b c d =
-  let ivar = Ivar_3.create () in
+  let ivar = Ivar_4.create () in
 
   let vtx_a = Vertex.create' @@ fun _ctx -> a () in
   let vtx_b = Vertex.create' @@ fun _ctx -> b () in
   let vtx_c = Vertex.create' @@ fun _ctx -> c () in
-  let vtx_d = Vertex.create' @@ fun ctx -> d () ; Ivar_3.notify ivar ctx in
+  let vtx_d = Vertex.create' @@ fun ctx -> d () ; Ivar_4.notify ivar ctx () in
 
   Vertex.precede vtx_a vtx_b ;
   Vertex.precede vtx_a vtx_c ;
