theories/zoo_parabs/future__code.v
@@ -6,35 +6,33 @@ From zoo.language Require Import
 From zoo_parabs Require Import
   pool.
 From zoo_std Require Import
-  lst
-  ivar_3.
+  ivar_4.
 From zoo_parabs Require Import
   future__types.
 From zoo Require Import
   options.
 
 Definition future_return : val :=
-  ivar_3_make.
+  ivar_4_make.
 
 Definition future_set : val :=
   fun: "ctx" "t" "res" =>
-    let: "waiters" := ivar_3_set "t" "res" in
-    lst_iter (fun: "waiter" => "waiter" "ctx" "res") "waiters".
+    ivar_4_notify "t" "ctx" "res".
 
 Definition future_async : val :=
   fun: "ctx" "task" =>
-    let: "t" := ivar_3_create () in
+    let: "t" := ivar_4_create () in
     pool_async "ctx" (fun: "ctx" => future_set "ctx" "t" ("task" "ctx")) ;;
     "t".
 
 Definition future_wait : val :=
   fun: "ctx" "t" =>
     pool_wait_ivar "ctx" "t" ;;
-    ivar_3_get "t".
+    ivar_4_get "t".
 
 Definition future_iter : val :=
   fun: "ctx" "t" "task" =>
-    match: ivar_3_wait "t" "task" with
+    match: ivar_4_wait "t" "task" with
     | None =>
         ()
     | Some "res" =>
@@ -43,7 +41,7 @@ Definition future_iter : val :=
 
 Definition future_map : val :=
   fun: "ctx" "t1" "task" =>
-    let: "t2" := ivar_3_create () in
+    let: "t2" := ivar_4_create () in
     future_iter
       "ctx"
       "t1"
