theories/zoo_std/ivar_3__opaque.v
@@ -9,4 +9,3 @@ From zoo_std Require Import
 #[global] Opaque ivar_3_get.
 #[global] Opaque ivar_3_wait.
 #[global] Opaque ivar_3_set.
-#[global] Opaque ivar_3_notify.
