theories/zoo_std/ivar_3__types.v
@@ -3,8 +3,6 @@ From zoo Require Import
 From zoo.language Require Import
   typeclasses
   notations.
-From zoo_std Require Import
-  lst.
 From zoo Require Import
   options.
 
